elle/ElleCorrect/ElleAltSemantics.thy
@@ -1,5 +1,5 @@
 theory ElleAltSemantics
-  imports Main "Valid4"
+  imports Main "Valid4" "../../EvmFacts" "../../example/termination/ProgramList"
 begin
 
 (*
@@ -188,6 +188,487 @@ next
 next
   case (11 i t cp x e h rest z z')
   then show ?case sorry
+qed
+
+fun clearprog_cctx :: "constant_ctx \<Rightarrow> constant_ctx" where
+"clearprog_cctx e =
+  (e \<lparr> cctx_program := empty_program \<rparr>)"
+
+(* TODO: be able to load at an arbitrary position (not just 0)? *)
+(* this one seems to have problems with reduction, so I'm not using it *)
+fun ll4_load_cctx :: "constant_ctx \<Rightarrow> ll4 \<Rightarrow> constant_ctx" where
+"ll4_load_cctx cc t =
+  (cc \<lparr> cctx_program := 
+        Evm.program_of_lst (codegen' t) ProgramInAvl.program_content_of_lst
+      \<rparr>)"
+
+(* based on ProgramList.program_list_of_lst *)
+fun  program_list_of_lst_validate  :: "inst list \<Rightarrow> inst list option"  where 
+ " program_list_of_lst_validate [] = Some []"
+|" program_list_of_lst_validate (Stack (PUSH_N bytes) # rest) =
+    (if length bytes \<le> 0 then None
+     else (if length bytes > 32 then None
+           else (case program_list_of_lst_validate rest of
+                        None \<Rightarrow> None
+                      | Some rest' \<Rightarrow> 
+                          Some ([Stack (PUSH_N bytes)] @
+                            map(\<lambda>x. Unknown x) bytes @ rest'))))"
+|" program_list_of_lst_validate (i # rest) = 
+    (case program_list_of_lst_validate rest of None \<Rightarrow> None | Some rest' \<Rightarrow> Some (i#rest'))"
+
+
+(* seeing if the list version is easier to work with *)
+(* this one doesn't seem to quite be what we want *)
+fun ll4_load_lst_map_cctx :: "constant_ctx \<Rightarrow> ll4 \<Rightarrow> constant_ctx" where
+"ll4_load_lst_map_cctx cc t =
+  (cc \<lparr> cctx_program := Evm.program_of_lst (codegen' t) (\<lambda> il i . program_map_of_lst 0 il (nat i)) \<rparr>)"
+
+fun ll4_load_lst_cctx :: "constant_ctx \<Rightarrow> ll4 \<Rightarrow> constant_ctx" where
+"ll4_load_lst_cctx cc t =
+  (cc \<lparr> cctx_program := 
+      Evm.program.make (\<lambda> i . index (program_list_of_lst (codegen' t)) (nat i))
+                       (length (program_list_of_lst (codegen' t)))\<rparr>)"
+
+fun ll4_load_lst_validate :: "constant_ctx \<Rightarrow> ll4 \<Rightarrow> constant_ctx option" where
+"ll4_load_lst_validate cc t =
+  (case codegen'_check t of None \<Rightarrow> None
+        | Some tc \<Rightarrow>
+          (case program_list_of_lst_validate tc of None \<Rightarrow> None
+            | Some l \<Rightarrow> Some (cc \<lparr> cctx_program := 
+                                    Evm.program.make (\<lambda> i . index l (nat i))
+                                    (length l) \<rparr>)))"
+
+lemma program_list_of_lst_validate_split [rule_format] :
+"(! b c . program_list_of_lst_validate (a @ b) = Some c \<longrightarrow>
+ (? a' . program_list_of_lst_validate a = Some a' \<and>
+  (? b' . program_list_of_lst_validate b = Some b' \<and>
+      c = a' @ b')))"
+proof(induction a)
+case Nil
+  then show ?case 
+    apply(auto)
+    done
+next
+  case (Cons a b)
+  then show ?case 
+    apply(auto)
+    apply(case_tac a, auto)
+                apply(simp split:Option.option.split_asm Option.option.split, auto)
+               apply(simp split:Option.option.split_asm Option.option.split, auto)
+              apply(simp split:Option.option.split_asm Option.option.split, auto)
+             apply(simp split:Option.option.split_asm Option.option.split, auto)
+            apply(simp split:Option.option.split_asm Option.option.split, auto)
+           apply(simp split:Option.option.split_asm Option.option.split, auto)
+          apply(simp split:Option.option.split_asm Option.option.split, auto)
+         apply(simp split:Option.option.split_asm Option.option.split, auto)
+        apply(simp split:Option.option.split_asm Option.option.split, auto)
+    apply(case_tac x10, auto)
+          apply(simp split:Option.option.split_asm Option.option.split, auto)
+
+         apply(case_tac x2, auto)
+        apply(simp split:Option.option.split_asm Option.option.split, auto)
+       apply(simp split:Option.option.split_asm Option.option.split, auto)
+      apply(simp split:Option.option.split_asm Option.option.split, auto)
+     apply(simp split:Option.option.split_asm Option.option.split, auto)
+    apply(simp split:Option.option.split_asm Option.option.split, auto)
+    done
+qed
+
+fun setpc_ir :: "instruction_result \<Rightarrow> nat \<Rightarrow> instruction_result" where
+"setpc_ir ir n =
+  irmap (\<lambda> v . v \<lparr> vctx_pc := (int n) \<rparr>) ir"
+
+(* this is the basic idea of the theorem statement
+the only thing we need to do is specify the precise
+relationship between states - i.e. relationship between the cp that the
+semantics is starting from and the pc that the program starts from *)
+(*
+additional assumption - we need to be valid3', and our first element of the
+qvalidity has to be 0
+*)
+(* program_sem_t appears to be way too slow to execute - perhaps better
+to switch back... *)
+(* prove this holds for any non-continuing final state
+(problem - will we need to make this hold inductively for non-final states?)
+(will we have a problem with the hardcoded zero start? maybe we need to
+subtract it from the final pc)
+ *)
+(*
+lemma elle_alt_correct :
+"elle_alt_sem ((0, sz), (t :: ll4t)) elle_interp cp (ir, cc, net) (ir', cc', net') \<Longrightarrow>
+ ((0, sz), t) \<in> ll_valid3' \<Longrightarrow>
+ ll4_validate_jump_targets [] ((0,sz),t) \<Longrightarrow>
+ program_sem_t (ll4_load_cctx cc ((0,sz),t)) net ir = ir2' \<Longrightarrow>
+ setpc_ir ir' 0 = setpc_ir ir2' 0
+"
+*)
+(* Should we use "erreq", which throws away the details of the error *)
+(* perhaps the issue is that we are sort of implicitly destructing on
+the three-tuple in this inductive statement *)
+(* est should probably be a record
+  fst \<rightarrow> instruction result
+  fst . snd \<rightarrow> cctx
+  snd . snd \<rightarrow> net
+*)
+
+(* need new predicates: isi2e and iscont *)
+
+fun isi2e :: "instruction_result \<Rightarrow> bool" where
+"isi2e (InstructionToEnvironment _ _ _) = True"
+| "isi2e _ = False"
+
+definition iscont :: "instruction_result \<Rightarrow> bool" where
+"iscont i = (\<not> (isi2e i) )"
+
+(* from examples/termination/RunList *)
+(*
+theorem program_content_first [simp] :
+  "program_map_of_lst 0 (a # lst) 0 = Some a"
+apply(cases a)
+apply(auto)
+apply(subst program_list_content_eq4)
+apply(cases "get_stack a")
+apply(auto)
+done
+*)
+
+(* need a couple lemmas about program_map_of_lst *)
+
+(* will it suffice to only consider computations that end in a successful result? 
+this seems sketchy, but I guess the idea is "computation suffixes"
+*)
+
+lemma qvalid_less' :
+"(((a, (t :: ('a, 'b, 'c, 'd, 'e, 'f, 'g) llt)) \<in> ll_valid_q) \<longrightarrow> fst a \<le> snd a) \<and>
+ ((((a1, a2), (l:: ('a, 'b, 'c, 'd, 'e, 'f, 'g) ll list)) \<in> ll_validl_q \<longrightarrow> a1 \<le> a2))
+"
+  apply(induction rule: ll_valid_q_ll_validl_q.induct, auto)
+  done
+
+lemma qvalid_less1 :
+"((a, (t :: ('a, 'b, 'c, 'd, 'e, 'f, 'g) llt)) \<in> ll_valid_q) \<Longrightarrow> fst a \<le> snd a"
+  apply(insert qvalid_less') apply(fastforce)
+  done
+
+lemma qvalid_less2 :
+"(x, (l :: ('a, 'b, 'c, 'd, 'e, 'f, 'g) ll list)) \<in> ll_validl_q \<Longrightarrow> fst x \<le> snd x"
+  apply(insert qvalid_less') apply(case_tac x)
+  apply(fastforce)
+  done
+
+(* we need to rule out invalid (too long/ too short)
+stack instructions *)
+(* need additional premise about validity of
+jump annotations *)
+lemma qvalid_codegen'_check' :
+  "(((a, (t :: ll4t)) \<in> ll_valid_q) \<longrightarrow> 
+      (! il1 . codegen'_check (a, t) = Some il1 \<longrightarrow>
+      (! il2 . program_list_of_lst_validate il1 = Some il2 \<longrightarrow>
+      snd a \<ge> fst a \<and> length (il2) = snd a - fst a))) \<and>
+ (((a1, a2), (l::  ll4 list)) \<in> ll_validl_q \<longrightarrow> 
+      (! ils . List.those (map codegen'_check l) = Some ils \<longrightarrow>
+      (! il . program_list_of_lst_validate (List.concat ils) = Some il  \<longrightarrow>
+        a2 \<ge> a1 \<and> length il = a2 - a1)))"
+proof(induction rule:ll_valid_q_ll_validl_q.induct)
+case (1 i x e)
+  then show ?case 
+    apply(auto)
+    apply(case_tac i, auto)
+    apply(case_tac x10, auto)
+    apply(simp split: if_split_asm)
+    done
+next
+  case (2 x d e)
+  then show ?case by auto
+next
+  case (3 x d e s)
+  then show ?case 
+    apply(auto)
+    done
+next
+  case (4 x d e s)
+  then show ?case
+    apply(auto)
+    done
+next
+  case (5 n l n' e)
+  then show ?case 
+    apply(auto)
+     apply(case_tac "those (map codegen'_check l)", auto)
+apply(case_tac "those (map codegen'_check l)", auto)
+    done
+next
+  case (6 n)
+  then show ?case
+    apply(auto)
+    done
+next
+  case (7 n h n' t n'')
+  then show ?case 
+    apply(auto)
+    apply(case_tac "codegen'_check ((n,n'), h)", auto)
+     apply(drule_tac program_list_of_lst_validate_split) apply(auto)
+    apply(case_tac "codegen'_check ((n, n'), h)", auto)
+    apply(drule_tac program_list_of_lst_validate_split) apply(auto)
+    done
+qed
+
+lemma qvalid_codegen'_check1 [rule_format]:
+  "(((a, (t :: ll4t)) \<in> ll_valid_q) \<longrightarrow> 
+      (! il1 . codegen'_check (a, t) = Some il1 \<longrightarrow>
+      (! il2 . program_list_of_lst_validate il1 = Some il2 \<longrightarrow>
+      snd a \<ge> fst a \<and> length (il2) = snd a - fst a)))"
+  apply(insert qvalid_codegen'_check')
+  apply(fastforce)
+  done
+
+(* TODO: use descend here? *)
+
+lemma qvalid_desc_bounded' :
+"((a, (t :: ('a, 'b, 'c, 'd, 'e, 'f, 'g) llt)) \<in> ll_valid_q \<longrightarrow>
+ (! cp nd nd' desc . ll_get_node (a, t) cp = Some ((nd, nd'), desc) \<longrightarrow>
+    nd \<ge> fst a \<and> nd' \<le> snd a)) \<and>
+  (((al, al'), (l :: ('a, 'b, 'c, 'd, 'e, 'f, 'g) ll list)) \<in> ll_validl_q \<longrightarrow>
+    (! n  ac ac' tc. n < length l \<longrightarrow> l ! n = ((ac, ac'), tc) \<longrightarrow>
+   (! cp nd nd' desc . 
+    ll_get_node ((ac, ac'), tc) cp = Some ((nd, nd'), desc) \<longrightarrow>
+    nd \<ge> al \<and> nd' \<le> al')))" 
+proof(induction rule:ll_valid_q_ll_validl_q.induct)
+case (1 i x e)
+  then show ?case apply(auto)
+     apply(case_tac cp, auto)
+    apply(case_tac cp, auto)
+    done
+next
+  case (2 x d e)
+  then show ?case 
+    apply(auto)
+         apply(case_tac cp, auto)
+    apply(case_tac cp, auto)
+    done
+next
+  case (3 x d e s)
+  then show ?case
+apply(auto)
+         apply(case_tac cp, auto)
+    apply(case_tac cp, auto)
+    done
+next
+  case (4 x d e s)
+  then show ?case
+apply(auto)
+         apply(case_tac cp, auto)
+    apply(case_tac cp, auto)
+    done
+next
+  case (5 n l n' e)
+  then show ?case apply(auto)
+     apply(case_tac cp, auto)
+     apply(frule_tac ll_get_node_len) apply(drule_tac x = a in spec) apply(auto)
+     apply(case_tac "index l a", auto)
+     apply(frule_tac "ll_get_node_child") apply(auto)
+    apply(case_tac cp, auto)
+    apply(frule_tac ll_get_node_len)
+    apply(drule_tac x = a in spec) apply(auto)
+    apply(case_tac "index l a", auto)
+    apply(frule_tac "ll_get_node_child", auto)
+    done
+next
+  case (6 n)
+  then show ?case by auto
+next
+  case (7 n h n' t n'')
+  then show ?case 
+    apply(clarify)
+    apply(case_tac na, auto)
+      apply(drule_tac x = cp in spec) apply(auto)
+      apply(drule_tac qvalid_less2, auto)
+
+     apply(drule_tac x = nat in spec) apply(auto)
+     apply(rotate_tac -1)
+     apply(drule_tac x = cp in spec, rotate_tac -1)
+     apply(auto)
+     apply(drule_tac qvalid_less1, auto)
+
+     apply(drule_tac x = nat in spec) apply(auto)
+     apply(rotate_tac -1)
+     apply(drule_tac x = cp in spec, rotate_tac -1)
+     apply(auto)
+
+done
+qed
+
+lemma valid3'_qvalid :
+"((x,t )  :: ('a, 'b, 'c, 'd, 'e) ll3') \<in> ll_valid3' \<Longrightarrow>
+  ((x, t) :: ('a, 'b, 'c, 'd, 'e) ll3') \<in> ll_valid_q"
+  apply(induction rule:ll_valid3'.induct)
+  apply(auto simp add:ll_valid_q_ll_validl_q.intros)
+  done
+
+(*
+idea: don't use program_map_of_lst?
+maybe just use program_list_of_lst with index?
+it would be nice to be able to use the "bang" notation,
+but maybe LemExtraDefs.index is the way to go?
+*)
+lemma elle_alt_correct :
+"elle_alt_sem ((t :: ll4)) intp cp est est' (* (ir, cc, net) (ir', cc', net') *) \<Longrightarrow>
+ (t \<in> ll_valid3' \<longrightarrow>
+  (! tend ttree . t = ((0, tend), ttree) \<longrightarrow>
+ ll4_validate_jump_targets [] t \<longrightarrow>
+ intp = elle_interp \<longrightarrow>
+ (! targstart targend tdesc . ll_get_node t cp = Some ((targstart, targend), tdesc) \<longrightarrow>
+   (! vi . fst est = InstructionContinue vi \<longrightarrow>
+   (! act vc venv fuel stopper . program_sem stopper
+               (ll4_load_lst_cctx (fst (snd est)) t) 
+               fuel (snd (snd est)) 
+(* is this arithmetic around fst (fst t) right? *)
+(* perhaps we need a secondary proof that validity implies
+that targstart will be greater than or equal to fst (fst t) *)
+               (setpc_ir (fst est) (targstart  (*- fst (fst t) *))) = 
+                   (* fuel can be arbitrary, but we require to compute to a final result *)
+                   InstructionToEnvironment act vc venv \<longrightarrow>
+                  (* the issue may have to do with distinguishing between errors? *)
+                  setpc_ir (fst est') 0 = setpc_ir (InstructionToEnvironment act vc venv) 0)))))"
+proof(induction rule:elle_alt_sem.induct)
+case (1 t cp x e i instD jmpD jmpiD labD st st')
+  then show ?case 
+    apply(clarify)
+    apply(subgoal_tac "(x, llt.L e i) = ((targstart, targend), tdesc)") apply(auto)
+
+    apply(case_tac fuel, auto)
+     apply(split Option.option.split_asm) apply(auto)
+      apply(split Option.option.split_asm) apply(auto)
+     apply(split Option.option.split_asm) apply(auto)
+     apply(simp split:if_split_asm) apply(auto)
+         apply(simp_all add:program.defs)
+
+
+(*
+another phrasing of the lemmas we need
+0 (DONE) valid3' implies q validity
+1. (DONE) length of (program_list_of_lst) of a valid tree is equal to its ending annotation
+2 (DONE). if we are descended from a valid root then our start \<ge> root's start and our end \<le> root's end
+*)
+(*
+lemma:
+- if we are valid
+- and we have a descendent at a certain location
+- then we will find 
+- 
+*)
+
+         apply(case_tac elle_interp) 
+         apply(simp add:elle_interp_def, clarify)
+    apply(clarsimp)
+ (* ok, we should do a proof sketch:
+1. map_of_lst t addr = get_by_addr t (addr - startloc t)
+2. need to say something else about program sem (but what?) *)
+(* use Hoare? *)
+    apply(case_tac "rev cp")
+          apply( auto)
+          apply(simp add:elle_interp_def, clarify)
+
+          apply(case_tac st, clarsimp)
+
+
+    apply(subst)
+    (* show a correspondence between elle_instD an program_sem? *)
+          (*
+(* old proof follows *)
+          apply(case_tac fuel, auto)
+     apply(split Option.option.split_asm)
+      apply(split Option.option.split_asm) apply(auto)
+     apply(split Option.option.split_asm) apply(auto)
+      (* this case should be easy because the map lookup will always succeed
+          *)
+    apply(simp add:Evm.program.defs)
+      apply(case_tac i, auto) apply(case_tac x10, auto)
+
+
+     apply(simp split:if_split_asm) apply(auto)
+    apply(simp split: Option.option.split_asm)
+
+          apply(case_tac i, auto) apply(case_tac x10, auto)
+      (*   apply(case_tac i, auto) apply(case_tac x10, auto)
+        apply(case_tac i, auto) apply(case_tac x10, auto)
+       apply(case_tac i, auto) apply(case_tac x10, auto)
+      apply(case_tac i, auto) apply(case_tac x10, auto)
+     apply(split if_split_asm) apply(clarsimp)                                                                                                                                                                                                                  
+apply(case_tac i, clarsimp) (* is this the right place to split on i? *)
+    apply(case_tac x1)
+    apply(simp_all add: elle_interp_def)
+      apply(clarsimp) apply(case_tac st, simp) apply(hypsubst)
+(* manageable-ish up to here. case tac on i next? *)
+
+                  apply(simp split: if_split_asm)
+(* here we could derive a contradiction from the fact
+that Unknown is not a valid instruction - but I think
+we can also do a proof that mirrors how the valid cases
+will look (e.g. stop) *)
+(* mostly manageable up to here *)
+                     apply(simp_all add:check_resources_def)
+    apply(clarsimp)
+    apply(case_tac x2a, clarsimp)
+                     apply(case_tac "vctx_stack vi", clarsimp)
+                      apply(case_tac st) apply(clarsimp)
+    apply(subgoal_tac "True")
+                 apply(case_tac i, clarsimp)
+                        apply(split if_split_asm) apply(clarsimp)
+    apply(simp)
+    apply(simp split: Option.option.split_asm)
+*)
+(*
+                        apply(case_tac st, clarsimp)
+
+                        apply(simp split: if_split_asm) 
+                        apply(simp_all)
+                        apply (simp_all add:check_resources_def)
+                        apply(case_tac x10, clarsimp) apply(hypsubst)
+                        apply(fastforce)
+                        apply(fastforce)
+                        apply(clarsimp)
+                        apply(case_tac x2a, clarsimp)
+                        apply(case_tac i, clarsimp) apply(hypsubst)
+                        apply(case_tac x2, clarsimp) apply(case_tac st, simp, hypsubst)
+    apply(simp split:if_split_asm) 
+                        apply(fastforce)
+
+    apply(subst check_resources_def)
+    apply(simp add:lookup.simps)
+    
+next
+  case (2 t cp x e i cp' instD jmpD jmpiD labD st st' st'')
+  then show ?case sorry
+next
+  case (3 t cp x e d instD jmpD jmpiD labD st st')
+  then show ?case sorry
+next
+  case (4 st'' t cp x e d cp' instD jmpD jmpiD labD st st')
+  then show ?case sorry
+next
+  case (5 xl el dl cp t cpre cj xj ej dj nj cl instD jmpD jmpiD labD st st' st'')
+  then show ?case sorry
+next
+  case (6 xl el dl cp' cp t cpre cj xj ej dj nj cl instD jmpD jmpiD labD st st' st'')
+  then show ?case sorry
+next
+  case (7 t cp x e d n instD jmpD jmpiD labD st st')
+  then show ?case sorry
+next
+  case (8 st'' t cp x e d n cp' instD jmpD jmpiD labD st st')
+  then show ?case sorry
+next
+  case (9 t cp x e i z)
+  then show ?case sorry
+next
+  case (10 t cp x e i cp' z z')
+  then show ?case sorry
+next
+  case (11 i t cp x e h rest z z')
+  then show ?case
+    apply(clarsimp)
+    sorry
 qed
 
 (*
